make the Iris branch live alongside the master branch and make it compile, but splitting a different version of definitions for Iris to use

theories/iris_base.v
@@ -7,7 +7,7 @@ Set Implicit Arguments.
 Unset Strict Implicit.
 Unset Printing Implicit Defensive.
 
-Require Import common operations datatypes datatypes_properties opsem interpreter binary_format_parser.
+Require Import common datatypes_iris datatypes_properties_iris.
 
 From stdpp Require Import gmap.
 From iris.proofmode Require Import tactics.
@@ -16,24 +16,26 @@ From iris.bi.lib Require Import fractional.
 From iris.base_logic.lib Require Export gen_heap proph_map gen_inv_heap.
 From iris.program_logic Require Export weakestpre total_weakestpre.
 
-Definition expr := host_expr.
-Definition val := host_value.
+Definition iris_expr := host_expr.
+Definition iris_val := host_value.
 (* Use gmap to specify the host variable store instead. *)
-Definition host_state := gmap id (option val).
+Definition host_state := gmap id (option iris_val).
 Definition state : Type := host_state * store_record * list host_value.
 Definition observation := unit. (* TODO: ??? *)
 
-Definition of_val (v : val) : expr := HE_value v.
+Definition of_val (v : iris_val) : iris_expr := HE_value v.
 
-Fixpoint to_val (e : expr) : option val :=
+Fixpoint to_val (e : iris_expr) : option iris_val :=
   match e with
   | HE_value v => Some v
   | _ => None
   end.
   
 (* https://softwarefoundations.cis.upenn.edu/qc-current/Typeclasses.html *)
-Global Instance val_eq_dec : EqDecision val.
-Proof. decidable_equality. Defined.
+Global Instance val_eq_dec : EqDecision iris_val.
+Proof.
+  decidable_equality.
+Defined.
 
 Lemma of_to_val e v : to_val e = Some v → of_val v = e.
 Proof.
