theories/extraction.v
@@ -1,6 +1,6 @@
 (** Extraction to OCaml. **)
 (* (C) M. Bodin, J. Pichon - see LICENSE.txt *)
-(*
+
 From Coq Require Extraction.
 
 From Wasm Require Import
@@ -26,4 +26,3 @@ Extraction "extract"
   PP
   DummyHost.
 
- *)
