theories/pp.v
@@ -9,7 +9,7 @@ Require BinNatDef.
 Require Import ansi list_extra.
 
 Open Scope string_scope.
-(*
+
 Section Host.
 
 Variable host_function : eqType.
@@ -437,4 +437,3 @@ End Show.
 
 End PP.
 
-*)
